examples/sess/proofmode.v
@@ -1,0 +1,475 @@
+(** This file contains the definitions of Actris's tactics for symbolic
+execution of message-passing programs. The API of these tactics is documented
+in the [README.md] file. The implementation follows the same pattern for the
+implementation of these tactics that is used in Iris. In addition, it uses a
+standard pattern using type classes to perform the normalization.
+
+In addition to the tactics for symbolic execution, this file defines the tactic
+[solve_proto_contractive], which can be used to automatically prove that
+recursive protocols are contractive. *)
+From iris.proofmode Require Import coq_tactics reduction spec_patterns.
+From iris.heap_lang Require Export proofmode notation.
+From actris Require Export channel.
+
+
+From stdpp Require Import base gmap.
+From mathcomp Require Import ssreflect.
+From stdpp Require Import namespaces.
+From iris.algebra Require Import agree auth csum gset gmap excl frac.
+From iris.algebra Require Import max_prefix_list.
+From iris.heap_lang Require Import notation proofmode.
+From cryptis Require Import lib term gmeta cryptis primitives tactics role.
+From cryptis.examples Require Import iso_dh gen_conn sess.
+(* From crypti *)
+(* From cryptis.examples.sess Require impl. *)
+(* From cryptis.examples.sess.proofs Require Import base. *)
+From actris.channel Require Import proto_model proto.
+From iris.heap_lang Require Import lib.spin_lock.
+From iris.bi Require Import telescopes.
+
+From iris.proofmode Require Import coq_tactics reduction spec_patterns.
+From iris.heap_lang Require Export proofmode notation.
+
+Notation iProto Σ := (iProto Σ term).
+Notation iMsg Σ := (iMsg Σ term).
+
+(** * Tactics for proving contractiveness of protocols *)
+Ltac f_dist_le :=
+  match goal with
+  | H : _ ≡{?n}≡ _ |- _ ≡{?n'}≡ _ => apply (dist_le n); [apply H|lia]
+  end.
+
+Ltac solve_proto_contractive :=
+  solve_proper_core ltac:(fun _ =>
+    first [f_contractive; simpl in * | f_equiv | f_dist_le]).
+
+(** * Normalization of protocols *)
+Class ActionDualIf (d : bool) (a1 a2 : action) :=
+  dual_action_if : a2 = if d then action_dual a1 else a1.
+Global Hint Mode ActionDualIf ! ! - : typeclass_instances.
+
+Global Instance action_dual_if_false a : ActionDualIf false a a := eq_refl.
+Global Instance action_dual_if_true_send : ActionDualIf true Send Recv := eq_refl.
+Global Instance action_dual_if_true_recv : ActionDualIf true Recv Send := eq_refl.
+
+Class ProtoNormalize {Σ} (d : bool) (p : iProto Σ)
+    (pas : list (bool * iProto Σ)) (q : iProto Σ) :=
+  proto_normalize :
+    ⊢ iProto_dual_if d p <++>
+        foldr (iProto_app ∘ uncurry iProto_dual_if) END%proto pas ⊑ q.
+Global Hint Mode ProtoNormalize ! ! ! ! - : typeclass_instances.
+Arguments ProtoNormalize {_} _ _%_proto _%_proto _%_proto.
+
+Notation ProtoUnfold p1 p2 := (∀ d pas q,
+  ProtoNormalize d p2 pas q → ProtoNormalize d p1 pas q).
+
+Class MsgNormalize {Σ} (d : bool) (m1 : iMsg Σ)
+    (pas : list (bool * iProto Σ)) (m2 : iMsg Σ) :=
+  msg_normalize a :
+    ProtoNormalize d (<a> m1) pas (<(if d then action_dual a else a)> m2).
+Global Hint Mode MsgNormalize ! ! ! ! - : typeclass_instances.
+Arguments MsgNormalize {_} _ _%_msg _%_msg _%_msg.
+
+Section classes.
+  Context `{!chanG Σ, !heapGS Σ}.
+  Implicit Types TT : tele.
+  Implicit Types p : iProto Σ.
+  Implicit Types m : iMsg Σ.
+  Implicit Types P : iProp Σ.
+
+  Lemma proto_unfold_eq p1 p2 : p1 ≡ p2 → ProtoUnfold p1 p2.
+  Proof. rewrite /ProtoNormalize=> Hp d pas q. by rewrite Hp. Qed.
+
+  Global Instance proto_normalize_done p : ProtoNormalize false p [] p | 0.
+  Proof. rewrite /ProtoNormalize /= right_id. auto. Qed.
+  Global Instance proto_normalize_done_dual p :
+    ProtoNormalize true p [] (iProto_dual p) | 0.
+  Proof. rewrite /ProtoNormalize /= right_id. auto. Qed.
+  Global Instance proto_normalize_done_dual_end :
+    ProtoNormalize (Σ:=Σ) true END [] END | 0.
+  Proof. rewrite /ProtoNormalize /= right_id iProto_dual_end. auto. Qed.
+
+  Global Instance proto_normalize_dual d p pas q :
+    ProtoNormalize (negb d) p pas q →
+    ProtoNormalize d (iProto_dual p) pas q.
+  Proof. rewrite /ProtoNormalize. by destruct d; rewrite /= ?involutive. Qed.
+
+  Global Instance proto_normalize_app_l d p1 p2 pas q :
+    ProtoNormalize d p1 ((d,p2) :: pas) q →
+    ProtoNormalize d (p1 <++> p2) pas q.
+  Proof.
+    rewrite /ProtoNormalize /=. rewrite assoc.
+    by destruct d; by rewrite /= ?iProto_dual_app.
+  Qed.
+
+  Global Instance proto_normalize_end d d' p pas q :
+    ProtoNormalize d p pas q →
+    ProtoNormalize d' END ((d,p) :: pas) q | 0.
+  Proof.
+    rewrite /ProtoNormalize /=.
+    destruct d'; by rewrite /= ?iProto_dual_end left_id.
+  Qed.
+
+  Global Instance proto_normalize_app_r d p1 p2 pas q :
+    ProtoNormalize d p2 pas q →
+    ProtoNormalize false p1 ((d,p2) :: pas) (p1 <++> q) | 0.
+  Proof. rewrite /ProtoNormalize /= => H. by iApply iProto_le_app. Qed.
+
+  Global Instance proto_normalize_app_r_dual d p1 p2 pas q :
+    ProtoNormalize d p2 pas q →
+    ProtoNormalize true p1 ((d,p2) :: pas) (iProto_dual p1 <++> q) | 0.
+  Proof. rewrite /ProtoNormalize /= => H. by iApply iProto_le_app. Qed.
+
+  Global Instance msg_normalize_base d v P p q pas :
+    ProtoNormalize d p pas q →
+    MsgNormalize d (MSG v {{ P }}; p) pas (MSG v {{ P }}; q).
+  Proof.
+    rewrite /MsgNormalize /ProtoNormalize=> H a.
+    iApply iProto_le_trans; [|by iApply iProto_le_base].
+    destruct d; by rewrite /= ?iProto_dual_message ?iMsg_dual_base
+      iProto_app_message iMsg_app_base.
+  Qed.
+
+  Global Instance msg_normalize_exist {A} d (m1 m2 : A → iMsg Σ) pas :
+    (∀ x, MsgNormalize d (m1 x) pas (m2 x)) →
+    MsgNormalize d (∃ x, m1 x) pas (∃ x, m2 x).
+  Proof.
+    rewrite /MsgNormalize /ProtoNormalize=> H a.
+    destruct d, a; simpl in *; rewrite ?iProto_dual_message ?iMsg_dual_exist
+      ?iProto_app_message ?iMsg_app_exist /=; iIntros (x); iExists x; first
+      [move: (H x Send); by rewrite ?iProto_dual_message ?iProto_app_message
+      |move: (H x Recv); by rewrite ?iProto_dual_message ?iProto_app_message].
+  Qed.
+
+  Global Instance proto_normalize_message d a1 a2 m1 m2 pas :
+    ActionDualIf d a1 a2 →
+    MsgNormalize d m1 pas m2 →
+    ProtoNormalize d (<a1> m1) pas (<a2> m2).
+  Proof. by rewrite /ActionDualIf /MsgNormalize /ProtoNormalize=> ->. Qed.
+
+  Global Instance proto_normalize_swap {TT1 TT2} d a m m'
+      (tv1 : TT1 -t> val) (tP1 : TT1 -t> iProp Σ) (tm1 : TT1 -t> iMsg Σ)
+      (tv2 : TT2 -t> val) (tP2 : TT2 -t> iProp Σ)
+      (tp : TT1 -t> TT2 -t> iProto Σ) pas :
+    ActionDualIf d a Recv →
+    MsgNormalize d m pas m' →
+    MsgTele m' tv1 tP1 (tele_bind (λ.. x1, <!> tele_app tm1 x1))%proto →
+    (∀.. x1, MsgTele (tele_app tm1 x1) tv2 tP2 (tele_app tp x1)) →
+    ProtoNormalize d (<a> m) pas (<!.. x2> MSG tele_app tv2 x2 {{ tele_app tP2 x2 }};
+                                  <?.. x1> MSG tele_app tv1 x1 {{ tele_app tP1 x1 }};
+                                  tele_app (tele_app tp x1) x2) | 1.
+  Proof.
+    rewrite /ActionDualIf /MsgNormalize /ProtoNormalize /MsgTele.
+    rewrite tforall_forall=> Ha Hm Hm' Hm''.
+    iApply iProto_le_trans; [iApply Hm|]. rewrite Hm' -Ha. clear Ha Hm Hm'.
+    iApply iProto_le_texist_elim_l; iIntros (x1).
+    iApply iProto_le_texist_elim_r; iIntros (x2).
+    rewrite !tele_app_bind Hm'' {Hm''}.
+    iApply iProto_le_trans;
+      [iApply iProto_le_base; iApply (iProto_le_texist_intro_l _ x2)|].
+    iApply iProto_le_trans;
+      [|iApply iProto_le_base; iApply (iProto_le_texist_intro_r _ x1)]; simpl.
+    iApply iProto_le_base_swap.
+  Qed.
+
+  Global Instance proto_normalize_choice d a1 a2 P1 P2 p1 p2 q1 q2 pas :
+    ActionDualIf d a1 a2 →
+    ProtoNormalize d p1 pas q1 → ProtoNormalize d p2 pas q2 →
+    ProtoNormalize d (iProto_choice a1 P1 P2 p1 p2) pas
+                     (iProto_choice a2 P1 P2 q1 q2).
+  Proof.
+    rewrite /ActionDualIf /ProtoNormalize=> -> H1 H2. destruct d; simpl.
+    - rewrite !iProto_dual_choice !iProto_app_choice.
+      iApply iProto_le_choice; iSplit; by iIntros "$".
+    - rewrite !iProto_app_choice. iApply iProto_le_choice; iSplit; by iIntros "$".
+  Qed.
+
+  (** Automatically perform normalization of protocols in the proof mode when
+  using [iAssumption] and [iFrame]. *)
+  Global Instance pointsto_proto_from_assumption q c p1 p2 :
+    ProtoNormalize false p1 [] p2 →
+    FromAssumption q (c ↣ p1) (c ↣ p2).
+  Proof.
+    rewrite /FromAssumption /ProtoNormalize /= right_id.
+    rewrite bi.intuitionistically_if_elim.
+    iIntros (?) "H". by iApply (iProto_pointsto_le with "H").
+  Qed.
+  Global Instance pointsto_proto_from_frame q c p1 p2 :
+    ProtoNormalize false p1 [] p2 →
+    Frame q (c ↣ p1) (c ↣ p2) True.
+  Proof.
+    rewrite /Frame /ProtoNormalize /= right_id.
+    rewrite bi.intuitionistically_if_elim.
+    iIntros (?) "[H _]". by iApply (iProto_pointsto_le with "H").
+  Qed.
+End classes.
+
+(** * Symbolic execution tactics *)
+(* TODO: Maybe strip laters from other hypotheses in the future? *)
+Lemma tac_wp_recv `{!chanG Σ, !heapGS Σ} {TT : tele} Δ i j K c p m tv tP tP' tp Φ :
+  envs_lookup i Δ = Some (false, c ↣ p)%I →
+  ProtoNormalize false p [] (<?> m) →
+  MsgTele m tv tP tp →
+  (∀.. x, MaybeIntoLaterN false 1 (tele_app tP x) (tele_app tP' x)) →
+  let Δ' := envs_delete false i false Δ in
+  (∀.. x : TT,
+    match envs_app false
+        (Esnoc (Esnoc Enil j (tele_app tP' x)) i (c ↣ tele_app tp x)) Δ' with
+    | Some Δ'' => envs_entails Δ'' (WP fill K (of_val (tele_app tv x)) {{ Φ }})
+    | None => False
+    end) →
+  envs_entails Δ (WP fill K (recv c) {{ Φ }}).
+Proof.
+  rewrite envs_entails_unseal /ProtoNormalize /MsgTele /MaybeIntoLaterN /=.
+  rewrite !tforall_forall right_id.
+  intros ? Hp Hm HP HΦ. rewrite envs_lookup_sound //; simpl.
+  assert (c ↣ p ⊢ c ↣ <?.. x>
+    MSG tele_app tv x {{ ▷ tele_app tP' x }}; tele_app tp x) as ->.
+  { iIntros "Hc". iApply (iProto_pointsto_le with "Hc"). iIntros "!>".
+    iApply iProto_le_trans; [iApply Hp|rewrite Hm].
+    iApply iProto_le_texist_elim_l; iIntros (x).
+    iApply iProto_le_trans; [|iApply (iProto_le_texist_intro_r _ x)]; simpl.
+    iIntros "H". by iDestruct (HP with "H") as "$". }
+  rewrite -wp_bind. eapply bi.wand_apply;
+    [by eapply bi.wand_entails, (recv_spec _ (tele_app tv) (tele_app tP') (tele_app tp))|f_equiv; first done].
+  rewrite -bi.later_intro; apply bi.forall_intro=> x.
+  specialize (HΦ x). destruct (envs_app _ _) as [Δ'|] eqn:HΔ'=> //.
+  rewrite envs_app_sound //; simpl. by rewrite right_id HΦ.
+Qed.
+
+Tactic Notation "wp_recv_core" tactic3(tac_intros) "as" tactic3(tac) :=
+  let solve_pointsto _ :=
+    let c := match goal with |- _ = Some (_, (?c ↣ _)%I) => c end in
+    iAssumptionCore || fail "wp_recv: cannot find" c "↣ ? @ ?" in
+  wp_pures;
+  let Hnew := iFresh in
+  lazymatch goal with
+  | |- envs_entails _ (wp ?s ?E ?e ?Q) =>
+    first
+      [reshape_expr e ltac:(fun K e' => eapply (tac_wp_recv _ _ Hnew K))
+      |fail 1 "wp_recv: cannot find 'recv' in" e];
+    [solve_pointsto ()
+       |tc_solve || fail 1 "wp_recv: protocol not of the shape <?>"
+    |tc_solve || fail 1 "wp_recv: cannot convert to telescope"
+    |tc_solve
+    |pm_reduce; simpl; tac_intros;
+     tac Hnew;
+     wp_finish]
+  | _ => fail "wp_recv: not a 'wp'"
+  end.
+
+Tactic Notation "wp_recv" "as" constr(pat) :=
+  wp_recv_core (idtac) as (fun H => iDestructHyp H as pat).
+
+Tactic Notation "wp_recv" "(" simple_intropattern_list(xs) ")" "as" constr(pat) :=
+  wp_recv_core (intros xs) as (fun H => iDestructHyp H as pat).
+Tactic Notation "wp_recv" "(" simple_intropattern_list(xs) ")" "as"
+    "(" ne_simple_intropattern_list(ys) ")" constr(pat) :=
+  wp_recv_core (intros xs) as (fun H => _iDestructHyp H ys pat).
+
+Lemma tac_wp_send `{!chanG Σ, !heapGS Σ} {TT : tele} Δ neg i js K c v p m tv tP tp Φ :
+  envs_lookup i Δ = Some (false, c ↣ p)%I →
+  ProtoNormalize false p [] (<!> m) →
+  MsgTele m tv tP tp →
+  let Δ' := envs_delete false i false Δ in
+  (∃.. x : TT,
+    match envs_split (if neg is true then base.Right else base.Left) js Δ' with
+    | Some (Δ1,Δ2) =>
+       match envs_app false (Esnoc Enil i (c ↣ tele_app tp x)) Δ2 with
+       | Some Δ2' =>
+          v = tele_app tv x ∧
+          envs_entails Δ1 (tele_app tP x) ∧
+          envs_entails Δ2' (WP fill K (of_val #()) {{ Φ }})
+       | None => False
+       end
+    | None => False
+    end) →
+  envs_entails Δ (WP fill K (send c v) {{ Φ }}).
+Proof.
+  rewrite envs_entails_unseal /ProtoNormalize /MsgTele /= right_id texist_exist.
+  intros ? Hp Hm [x HΦ]. rewrite envs_lookup_sound //; simpl.
+  destruct (envs_split _ _ _) as [[Δ1 Δ2]|] eqn:? => //.
+  destruct (envs_app _ _ _) as [Δ2'|] eqn:? => //.
+  rewrite envs_split_sound //; rewrite (envs_app_sound Δ2) //; simpl.
+  destruct HΦ as (-> & -> & ->). rewrite right_id assoc.
+  assert (c ↣ p ⊢
+    c ↣ <!.. (x : TT)> MSG tele_app tv x {{ tele_app tP x }}; tele_app tp x) as ->.
+  { iIntros "Hc". iApply (iProto_pointsto_le with "Hc"); iIntros "!>".
+    iApply iProto_le_trans; [iApply Hp|]. by rewrite Hm. }
+  eapply bi.wand_apply; [rewrite -wp_bind; by eapply bi.wand_entails, send_spec_tele|].
+  by rewrite -bi.later_intro.
+Qed.
+
+Tactic Notation "wp_send_core" tactic3(tac_exist) "with" constr(pat) :=
+  let solve_pointsto _ :=
+    let c := match goal with |- _ = Some (_, (?c ↣ _)%I) => c end in
+    iAssumptionCore || fail "wp_send: cannot find" c "↣ ? @ ?" in
+  let solve_done d :=
+    lazymatch d with
+    | true =>
+       done ||
+       let Q := match goal with |- envs_entails _ ?Q => Q end in
+       fail "wp_send: cannot solve" Q "using done"
+    | false => idtac
+    end in
+  lazymatch spec_pat.parse pat with
+  | [SGoal (SpecGoal GSpatial ?neg ?Hs_frame ?Hs ?d)] =>
+     let Hs' := eval cbv in (if neg then Hs else Hs_frame ++ Hs) in
+     wp_pures;
+     lazymatch goal with
+     | |- envs_entails _ (wp ?s ?E ?e ?Q) =>
+       first
+         [reshape_expr e ltac:(fun K e' => eapply (tac_wp_send _ neg _ Hs' K))
+         |fail 1 "wp_send: cannot find 'send' in" e];
+       [solve_pointsto ()
+       |tc_solve || fail 1 "wp_send: protocol not of the shape <!>"
+       |tc_solve || fail 1 "wp_send: cannot convert to telescope"
+       |pm_reduce; simpl; tac_exist;
+        repeat lazymatch goal with
+        | |- ∃ _, _ => eexists _
+        end;
+        lazymatch goal with
+        | |- False => fail "wp_send:" Hs' "not found"
+        | _ => notypeclasses refine (conj (eq_refl _) (conj _ _));
+                [iFrame Hs_frame; solve_done d
+                |wp_finish]
+        end]
+     | _ => fail "wp_send: not a 'wp'"
+     end
+  | _ => fail "wp_send: only a single goal spec pattern supported"
+  end.
+
+Tactic Notation "wp_send" "with" constr(pat) :=
+  wp_send_core (idtac) with pat.
+Tactic Notation "wp_send" "(" ne_uconstr_list(xs) ")" "with" constr(pat) :=
+  wp_send_core (ltac1_list_iter ltac:(fun x => eexists x) xs) with pat.
+
+Lemma tac_wp_branch `{!chanG Σ, !heapGS Σ} Δ i j K
+    c p P1 P2 (p1 p2 : iProto Σ) Φ :
+  envs_lookup i Δ = Some (false, c ↣ p)%I →
+  ProtoNormalize false p [] (p1 <{P1}&{P2}> p2) →
+  let Δ' := envs_delete false i false Δ in
+  (∀ b : bool,
+    match envs_app false
+        (Esnoc (Esnoc Enil j (if b then P1 else P2)) i (c ↣ (if b then p1 else p2))) Δ' with
+    | Some Δ'' => envs_entails Δ'' (WP fill K (of_val #b) {{ Φ }})
+    | None => False
+    end) →
+  envs_entails Δ (WP fill K (recv c) {{ Φ }}).
+Proof.
+  rewrite envs_entails_unseal /ProtoNormalize /= right_id=> ? Hp HΦ.
+  rewrite envs_lookup_sound //; simpl.
+  rewrite (iProto_pointsto_le _ _ (p1 <{P1}&{P2}> p2)%proto) -bi.later_intro -Hp left_id.
+  rewrite -wp_bind. eapply bi.wand_apply; [by eapply bi.wand_entails, branch_spec|f_equiv; first done].
+  rewrite -bi.later_intro; apply bi.forall_intro=> b.
+  specialize (HΦ b). destruct (envs_app _ _) as [Δ'|] eqn:HΔ'=> //.
+  rewrite envs_app_sound //; simpl. by rewrite right_id HΦ.
+Qed.
+
+Tactic Notation "wp_branch_core" "as" tactic3(tac1) tactic3(tac2) :=
+  let solve_pointsto _ :=
+    let c := match goal with |- _ = Some (_, (?c ↣ _)%I) => c end in
+    iAssumptionCore || fail "wp_branch: cannot find" c "↣ ? @ ?" in
+  wp_pures;
+  let Hnew := iFresh in
+  lazymatch goal with
+  | |- envs_entails _ (wp ?s ?E ?e ?Q) =>
+    first
+      [reshape_expr e ltac:(fun K e' => eapply (tac_wp_branch _ _ Hnew K))
+      |fail 1 "wp_branch: cannot find 'recv' in" e];
+    [solve_pointsto ()
+       |tc_solve || fail 1 "wp_send: protocol not of the shape <&>"
+    |pm_reduce; intros []; [tac1 Hnew|tac2 Hnew]; wp_finish]
+  | _ => fail "wp_branch: not a 'wp'"
+  end.
+
+Tactic Notation "wp_branch" "as" constr(pat1) "|" constr(pat2) :=
+  wp_branch_core as (fun H => iDestructHyp H as pat1) (fun H => iDestructHyp H as pat2).
+Tactic Notation "wp_branch" "as" "%" simple_intropattern(pat1) "|" constr(pat2) :=
+  wp_branch_core as (fun H => iPure H as pat1) (fun H => iDestructHyp H as pat2).
+Tactic Notation "wp_branch" "as" constr(pat1) "|" "%" simple_intropattern(pat2) :=
+  wp_branch_core as (fun H => iDestructHyp H as pat1) (fun H => iPure H as pat2).
+Tactic Notation "wp_branch" "as" "%" simple_intropattern(pat1) "|" "%" simple_intropattern(pat2) :=
+  wp_branch_core as (fun H => iPure H as pat1) (fun H => iPure H as pat2).
+Tactic Notation "wp_branch" := wp_branch as % _ | % _.
+
+Lemma tac_wp_select `{!chanG Σ, !heapGS Σ} Δ neg i js K
+    c (b : bool) p P1 P2 (p1 p2 : iProto Σ) Φ :
+  envs_lookup i Δ = Some (false, c ↣ p)%I →
+  ProtoNormalize false p [] (p1 <{P1}+{P2}> p2) →
+  let Δ' := envs_delete false i false Δ in
+  match envs_split (if neg is true then base.Right else base.Left) js Δ' with
+  | Some (Δ1,Δ2) =>
+     match envs_app false (Esnoc Enil i (c ↣ if b then p1 else p2)) Δ2 with
+     | Some Δ2' =>
+        envs_entails Δ1 (if b then P1 else P2) ∧
+        envs_entails Δ2' (WP fill K (of_val #()) {{ Φ }})
+     | None => False
+     end
+  | None => False
+  end →
+  envs_entails Δ (WP fill K (send c #b) {{ Φ }}).
+Proof.
+  rewrite envs_entails_unseal /ProtoNormalize /= right_id=> ? Hp HΦ.
+  rewrite envs_lookup_sound //; simpl.
+  rewrite (iProto_pointsto_le _ _ (p1 <{P1}+{P2}> p2)%proto) -bi.later_intro -Hp left_id.
+  rewrite -wp_bind. eapply bi.wand_apply; [by eapply bi.wand_entails, select_spec|].
+  rewrite -assoc; f_equiv; first done.
+  destruct (envs_split _ _ _) as [[Δ1 Δ2]|] eqn:? => //.
+  destruct (envs_app _ _ _) as [Δ2'|] eqn:? => //.
+  rewrite envs_split_sound //; rewrite (envs_app_sound Δ2) //; simpl.
+  destruct HΦ as [-> ->]. by rewrite -bi.later_intro right_id.
+Qed.
+
+Tactic Notation "wp_select" "with" constr(pat) :=
+  let solve_pointsto _ :=
+    let c := match goal with |- _ = Some (_, (?c ↣ _)%I) => c end in
+    iAssumptionCore || fail "wp_select: cannot find" c "↣ ? @ ?" in
+  let solve_done d :=
+    lazymatch d with
+    | true =>
+       done ||
+       let Q := match goal with |- envs_entails _ ?Q => Q end in
+       fail "wp_select: cannot solve" Q "using done"
+    | false => idtac
+    end in
+  lazymatch spec_pat.parse pat with
+  | [SGoal (SpecGoal GSpatial ?neg ?Hs_frame ?Hs ?d)] =>
+     let Hs' := eval cbv in (if neg then Hs else Hs_frame ++ Hs) in
+     wp_pures;
+     lazymatch goal with
+     | |- envs_entails _ (wp ?s ?E ?e ?Q) =>
+       first
+         [reshape_expr e ltac:(fun K e' => eapply (tac_wp_select _ neg _ Hs' K))
+         |fail 1 "wp_select: cannot find 'send' in" e];
+       [solve_pointsto ()
+       |tc_solve || fail 1 "wp_select: protocol not of the shape <+>"
+       |pm_reduce;
+        lazymatch goal with
+        | |- False => fail "wp_select:" Hs' "not fresh"
+        | _ => notypeclasses refine (conj _ _); [iFrame Hs_frame; solve_done d|wp_finish]
+        end]
+     | _ => fail "wp_select: not a 'wp'"
+     end
+  | _ => fail "wp_select: only a single goal spec pattern supported"
+  end.
+
+Tactic Notation "wp_select" := wp_select with "[//]".
+
+Tactic Notation "wp_new_chan" constr(prot) "as"
+       "(" simple_intropattern(c1) simple_intropattern(c2) ")" constr(pat) :=
+  wp_smart_apply (new_chan_spec prot); [done|];
+  iIntros (c1); iIntros (c2); iIntros pat.
+
+Tactic Notation "wp_fork_chan" constr(prot) "as"
+       simple_intropattern(c1) constr(pat1) "and"
+       simple_intropattern(c2) constr(pat2) :=
+  wp_smart_apply (fork_chan_spec prot); [iIntros (c2); iIntros pat2|
+                                         iIntros (c1); iIntros pat1].
+
+Tactic Notation "wp_fork_chan" constr(prot) "as"
+       simple_intropattern(c) constr(pat) :=
+  wp_fork_chan prot as c pat and c pat.
+
+Tactic Notation "wp_fork_chan" constr(prot) :=
+  wp_fork_chan prot as ? "?".
